ConNF/Model.lean
@@ -3,3 +3,4 @@ import ConNF.Model.Construction
 import ConNF.Model.BasePositions
 import ConNF.Model.Redefinitions
 import ConNF.Model.Basic
+import ConNF.Model.Hailperin
